\documentclass[UTF8]{ctexart}
\usepackage{ctex}
\usepackage{amsmath}
\title{电动力学-第一次作业}
\author{吴远清-2018300001031}
\begin{document}
	\maketitle
	1.11 Find the gradients of the following functions:\\
	(a)$f(x,y,z) = x^2 + y^3 + z^4$\\
	(b)$f(x,y,z) = x^2y^3z^4$\\
	(c)$f(x,y,z) = e^x sin(y) ln(z)$\\
	Answer:\\
	(a):
	$$\nabla f = 2x\hat{x} + 3 y^2 \hat{y} + 4z^3 \hat{z} \eqno(1.1)$$
	(b):
	$$\nabla f = 2x y^3 z^4 \hat{x} + 3 x^2 y^2 z^4 \hat{y} + 4 x^2 y^3 z^3 \hat{z} \eqno(1.2)$$
	(c):
	$$\nabla f = e^x sin(y) ln(z) \hat{x} + e^x cos(y) ln(z) \hat{y} + \frac{e^x sin(y)}{z} \hat{z} \eqno(1.1)$$
	1.15 Calculate the divergence of the following vector functions:\\
	(a)$V_a = x^2 \hat{x} + 3 x z^2 \hat{y} - 2 x z \hat{z}$\\
	(b)$V_b = x y \hat{x} + 2 y z \hat{y} + 3 z x \hat{z}$\\
	(c)$V_c = y^2 \hat{x} + (2 x y + z^2) \hat{y} + 2 y z \hat{z}$\\
	Answe:\\
	(a):\\
	$$\nabla \cdot V_a = 2 x - 2 x = 0 \eqno(2.1)$$
	(b):\\
	$$\nabla \cdot V_b = y + 2 z + 3x \eqno(2.2)$$
	(c):
	$$\nabla \cdot V_c = 2 x + 2 y \eqno(2.3)$$
	1.18 Calculate the curls of the vector functions in Prob. 1.15.\\
	Answer:\\
	(a)\\
	$$\nabla \times V_a = \left |\begin{array}{cccc}
	\hat{x} & \hat{y} & \hat{z}\\
	\partial/\partial x & \partial/\partial y & \partial/\partial z \\
	x^2 & 3 x z^2 & -2 x z
	\end{array}\right | = -6xz\hat{x} + 2 z \hat{y} + 3z^2\hat{z} \eqno(3.1)$$
	(b):\\
	$$\nabla \times V_b = \left |\begin{array}{cccc}
	\hat{x} & \hat{y} & \hat{z}\\
	\partial/\partial x & \partial/\partial y & \partial/\partial z \\
	xy & 2yz & 3zx
	\end{array}\right | = -2y\hat{x} + -3z \hat{y} + -x\hat{z} \eqno(3.1)$$
	(c):\\
	$$\nabla \times V_b = \left |\begin{array}{cccc}
	\hat{x} & \hat{y} & \hat{z}\\
	\partial/\partial x & \partial/\partial y & \partial/\partial z \\
	x^2 & 3 x z^2 & -2 x z
	\end{array}\right | =0 \eqno(3.3)$$
	1.36\\
	(a) Show that:
	$$\int_S f(\nabla \times A) \cdot da = \int_S[A\times(\nabla f)]\cdot da + \oint_PfA\cdot dl$$
	(b) Show that:
	$$\int_v B\cdot(\nabla \times A)d\tau = \int_v A \cdot (\nabla \times B)d\tau + \oint_S (A \times B)\cdot da$$
	Answer:
	(a) According to the product rules:
	$$f(\nabla \times A) = \nabla \times (fA) + A \times (\nabla f) \eqno(4.1.1)$$
	So, the integrate transform to:
	$$\int_Sf(\nabla \times A)\cdot da = \int_S[A \times (\nabla f)]\cdot da + \int_S\nabla \times (fA)\cdot da \eqno(4.1.2)$$
	And using Stokes theorem:
	$$\int_S[\nabla \times (fA)] \cdot da = \oint_PfA\cdot dl \eqno(4.1.3)$$
	So, we get:
	$$\int_S f(\nabla \times A) \cdot da = \int_S[A\times(\nabla f)]\cdot da + \oint_PfA\cdot dl \eqno(4.1.4)$$
	Q.E.D\\
	(b):\\
	Similarly, according to the product rules:
	$$B \cdot (\nabla \times A) = A \cdot (\nabla \times B) + \nabla \cdot (A \times B) \eqno(4.2.1)$$
	According to the equation (4.2.1), the left side of the equation to be proved could be transform to:
	$$\int_v B \cdot (\nabla \times A)\cdot d\tau = \int_v A \cdot (\nabla \times B)\cdot d\tau + \int_v \nabla \cdot (A \times B) \cdot d\tau \eqno(4.2.2)$$
	Then, using the Green theorem:
	$$\int_v \nabla \cdot (A \times B) \cdot d\tau = \int_S(a \times B)\cdot da \eqno(4.2.3)$$
	So, we get:
	$$\int_v B\cdot(\nabla \times A)d\tau = \int_v A \cdot (\nabla \times B)d\tau + \oint_S (A \times B)\cdot da \eqno(4.2.4)$$
	Q.E.D
	
\end{document}